theories/TM/L/CompilerBoolFuns/Compiler.v
@@ -7,7 +7,7 @@ Import Vector.VectorNotations ListNotations.
 
 From Undecidability.TM Require Import TM_facts ProgrammingTools WriteValue CaseList Copy ListTM Hoare.
 From Undecidability.TM.L Require Import Alphabets Eval.
-From Undecidability.TM.L.CompilerBoolFuns Require Import Compiler_spec Compiler_facts ClosedLAdmissible.
+From Undecidability.TM.L.CompilerBoolFuns Require Import Compiler_spec Compiler_facts.
 
 Require Import Equations.Prop.DepElim.
 
@@ -455,12 +455,12 @@ Proof.
   dependent destruct v. reflexivity.
 Qed.
 
-Theorem compiler_bool {k} (R : Vector.t (list bool) k -> (list bool) -> Prop) :
-  L_booL_bool_computable_closed R -> TM_booL_bool_computable R.
+Theorem compiler_bool_closed {k} (R : Vector.t (list bool) k -> (list bool) -> Prop) :
+  L_bool_computable_closed R -> TM_bool_computable R.
 Proof.
   intros H. 
-  eapply TM_booL_bool_computable_hoare'_spec.
-  { eapply L_bool_computable_function. now apply L_booL_bool_computable_can_closed. }
+  eapply TM_bool_computable_hoare'_spec.
+  { eapply L_bool_computable_function. now apply L_bool_computable_can_closed. }
   destruct H as [sim [cs Hsim]].
   hnf. 
   eexists _, _, sym_s, sym_b. split. eapply syms_diff. exists (M_main k sim).
