theories/TM/L/CompilerBoolFuns/LComp_to_TMComp.v
@@ -1,0 +1,4 @@
+From Undecidability.TM.L.CompilerBoolFuns Require Import Compiler_spec Compiler ClosedLAdmissible.
+
+Lemma L_computable_is_TM_computable f :
+  
